DeepWiki/SymbolicIntegration/Computable.lean
@@ -29,6 +29,7 @@ import DeepWiki.SymbolicIntegration.Computable.RischTowerPrimitive
 import DeepWiki.SymbolicIntegration.Computable.RischTowerPrimitiveLrt
 import DeepWiki.SymbolicIntegration.Computable.LrtAssembly
 import DeepWiki.SymbolicIntegration.Computable.RischSolverTower
+import DeepWiki.SymbolicIntegration.Computable.LrtCompleteness
 import DeepWiki.SymbolicIntegration.Computable.IntegratorCompleteness
 import DeepWiki.SymbolicIntegration.Computable.LinearSolveCorrect
 import DeepWiki.SymbolicIntegration.Computable.ListDet
